lib/misc.v
@@ -21,5 +21,17 @@ Definition node_lt (x y: node_rep) : Prop :=
 Definition rep_to_node (n: node_rep) : val :=
   (#(node_key n), oloc_to_val (node_next n), (node_lock n)).
 
-Definition key_equiv (S: gset node_rep) (S_keys: gset Z) :=
-  Permutation (elements S_keys) (map node_key (elements S)).
+Definition key_equiv (S: gset node_rep) (Skeys: gset Z) :=
+  Permutation (elements Skeys) (map node_key (elements S)).
+
+Fixpoint Zset_inclusive_range (z: Z) (gap : nat) : gset Z :=
+  match gap with
+  | O => {[ z ]}
+  | S n' => {[ z + S n']} ∪ (Zset_inclusive_range z n')
+  end.
+
+Definition Zset_exclusive_range (z: Z) (gap: nat) : gset Z :=
+  Zset_inclusive_range z gap ∖  {[ z; z + gap ]}.
+
+Definition Zlt_range (z1 z2: Z) : gset Z := 
+  Zset_exclusive_range z1 (Z.to_nat (z2 - z1)).
